removed Root from gbuffer; fixed Lib.PrintBuffer

lib/c/Lib_PrintBuffer.c
@@ -23,12 +23,10 @@ void Lib_PrintBuffer_print_compare(uint32_t len, uint8_t* buffer1, uint8_t* buff
   printf("\n");
 }
 
-void Lib_PrintBuffer_print_compare_display(uint8_t t1, uint8_t t2, uint32_t len, void* buf1, void* buf2) {
-  uint8_t* buffer1 = (uint8_t*) buf1;
-  uint8_t* buffer2 = (uint8_t*) buf2;
+void Lib_PrintBuffer_print_compare_display(uint32_t len, const uint8_t* buffer1, const uint8_t* buffer2) {
   uint8_t res = 0;
   uint32_t i;
-  Lib_PrintBuffer_print_compare(len, buffer1, buffer2);
+  Lib_PrintBuffer_print_compare(len, (uint8_t*)buffer1, (uint8_t*)buffer2);
   for (i = 0; i < len; i++) {
     res |= buffer1[i] ^ buffer2[i];
   }
@@ -40,12 +38,10 @@ void Lib_PrintBuffer_print_compare_display(uint8_t t1, uint8_t t2, uint32_t len,
   printf("\n");
 }
 
-bool Lib_PrintBuffer_result_compare_display(uint8_t t1, uint8_t t2, uint32_t len, void* buf1, void* buf2) {
-  uint8_t* buffer1 = (uint8_t*) buf1;
-  uint8_t* buffer2 = (uint8_t*) buf2;
+bool Lib_PrintBuffer_result_compare_display(uint32_t len, const uint8_t* buffer1, const uint8_t* buffer2) {
   uint8_t res = 0;
   uint32_t i;
-  Lib_PrintBuffer_print_compare(len, buffer1, buffer2);
+  Lib_PrintBuffer_print_compare(len, (uint8_t*)buffer1, (uint8_t*)buffer2);
   for (i = 0; i < len; i++) {
     res |= buffer1[i] ^ buffer2[i];
   }
