lib/Lib.PrintBuffer.fsti
@@ -22,21 +22,17 @@ val print_compare:
   (ensures (fun h0 _ h1 -> modifies0 h0 h1))
 
 val print_compare_display:
-    #t1: buftype
-  -> #t2: buftype
-  -> len: size_t
-  -> buf0: lbuffer_t t1 uint8 len
-  -> buf1: lbuffer_t t2 uint8 len ->
+     len: size_t
+  -> buf0: clbuffer uint8 len
+  -> buf1: clbuffer uint8 len ->
   Stack unit
   (requires (fun h -> live h buf0 /\ live h buf1))
   (ensures (fun h0 _ h1 -> modifies0 h0 h1))
 
 val result_compare_display:
-    #t1: buftype
-  -> #t2: buftype
-  -> len: size_t
-  -> buf0: lbuffer_t t1 uint8 len
-  -> buf1: lbuffer_t t2 uint8 len ->
+     len: size_t
+  -> buf0: clbuffer uint8 len
+  -> buf1: clbuffer uint8 len ->
   Stack bool
   (requires (fun h -> live h buf0 /\ live h buf1))
   (ensures (fun h0 _ h1 -> modifies0 h0 h1))
